lib/logger.ml
@@ -1,0 +1,71 @@
+module Logger = struct 
+
+  type t = string list
+  let init : t = []
+
+  let add_msg (x : t) (txt : string) : t = 
+    x @ [txt]
+
+  let sub s = 
+    let len = 55 in
+    if String.length s >= len then (String.sub s 0 len)  ^ " ... ... "
+    else s
+
+  let enter_module (x : t) (mod_name : string) : t =
+    add_msg
+      x
+      (Printf.sprintf "[Module] %s\n" mod_name)
+
+  let enter_action (x : t) (pred_name : string) : t = 
+    add_msg 
+      x 
+      (Printf.sprintf "[Action] %s" pred_name)
+
+  let error_then_else_not_assigning_same_set_of_vars
+    (x : t) (expr_str : string) : t =
+    add_msg
+      x 
+      (Printf.sprintf 
+        "Then-branch and else-branch do not assign the same set of variables: \n\t%s\n"
+        (sub expr_str))
+
+  let error_lft_expr_not_output (x : t) (expr_str : string) : t = 
+    add_msg
+      x 
+      (Printf.sprintf 
+        "This expr on the left side of an equivalence is not an output-mode variable: %s\n"
+        expr_str)
+
+  let error_output_used_but_not_assigned
+    (x : t) (expr_str : string) : t =
+    add_msg 
+      x 
+      (Printf.sprintf
+        "This expr contains an output-mode variable that is \n\tnot assigned in the previous context:\n\t%s\n"
+        (sub expr_str))
+    
+  let error_saturation_check_failed
+    (x : t) : t = 
+    add_msg 
+      x 
+      "Saturation check failed: Output-mode variables are not fully assigned\n"
+
+  let error_harmony_check_failed
+    (x : t) (expr_str : string) : t = 
+    add_msg 
+      x 
+      (Printf.sprintf
+        "Harmony check failed: \n\tThis output-mode variable has been assigned multiple times: \n\t\t%s\n"
+        expr_str)
+
+  let error_none
+    (x : t) : t = 
+    add_msg x "Check passed\n"
+
+  let print (x : t) : string = 
+    "/**********************************************************************" ^ "\n" ^
+    "AUTOMAN LOG" ^ "\n\n" ^
+    (String.concat "\n" x) ^ 
+    "**********************************************************************/" ^ "\n\n"
+
+end
