asset/impl/KV/Parameters.i.dfy
@@ -1,1 +1,34 @@
-Error: TopLevel.find_module: not found: (Internal.NonEmptyList.:: ("Protocol_Parameters_i", []))
+/**********************************************************************
+AUTOMAN LOG
+
+[Module] Protocol_Parameters_i
+**********************************************************************/
+
+include ""
+
+
+module Impl_Protocol_Parameters_i 
+{
+
+	datatype CParameters = 
+	CParameters(
+		max_seqno: nat, 
+		max_delegations: nat
+	)
+
+	predicate CParametersIsValid(s: CParameters) 
+	{
+		CParametersIsAbstractable(s)
+	}
+
+	predicate CParametersIsAbstractable(s: CParameters) 
+	{
+		true
+	}
+
+	function AbstractifyCParametersToParameters(s: CParameters) : Parameters 
+		requires CParametersIsAbstractable(s)
+	{
+		Parameters(s.max_seqno, s.max_delegations)
+	}
+}
