asset/impl/KV/SingleMessage.i.dfy
@@ -1,1 +1,55 @@
-Error: TopLevel.find_module: not found: (Internal.NonEmptyList.:: ("SHT__SingleMessage_i", []))
+/**********************************************************************
+AUTOMAN LOG
+
+[Module] SHT__SingleMessage_i
+**********************************************************************/
+
+include ""
+
+
+module Impl_SHT__SingleMessage_i 
+{
+
+	datatype CSingleMessage = 
+	CSingleMessage(
+		seqno: nat, 
+		dst: EndPoint, 
+		m: CMessage
+	)
+	 | 
+	CAck(
+		ack_seqno: nat
+	)
+	 | 
+	CInvalidMessage(
+		
+	)
+
+	predicate CSingleMessageIsValid(s: CSingleMessage) 
+	{
+		match s
+		case CSingleMessage(seqno, dst, m) => CSingleMessageIsAbstractable(s) && EndPointIsValid(s.dst) && CMessageIsValid(s.m)
+		case CAck(ack_seqno) => CSingleMessageIsAbstractable(s)
+		case CInvalidMessage() => CSingleMessageIsAbstractable(s)
+
+	}
+
+	predicate CSingleMessageIsAbstractable(s: CSingleMessage) 
+	{
+		match s
+		case CSingleMessage(seqno, dst, m) => EndPointIsAbstractable(s.dst) && CMessageIsAbstractable(s.m)
+		case CAck(ack_seqno) => true
+		case CInvalidMessage() => true
+
+	}
+
+	function AbstractifyCSingleMessageToSingleMessage(s: CSingleMessage) : SingleMessage 
+		requires CSingleMessageIsAbstractable(s)
+	{
+		match s
+		case CSingleMessage(seqno, dst, m) => SingleMessage(s.seqno, AbstractifyEndPointToNodeIdentity(s.dst), AbstractifyCMessageToMessage(s.m))
+		case CAck(ack_seqno) => Ack(s.ack_seqno)
+		case CInvalidMessage() => InvalidMessage()
+
+	}
+}
