asset/impl/BadExamples/Acceptor.i.dfy
@@ -1,0 +1,119 @@
+/**********************************************************************
+AUTOMAN LOG
+
+[Module] LiveRSL__Acceptor_i
+
+[Action] LAcceptorInit
+Saturation check failed: Output-mode variables are not fully assigned
+
+[Action] RemoveVotesBeforeLogTruncationPoint
+Saturation check failed: Output-mode variables are not fully assigned
+
+[Action] LAcceptorProcessHeartbeat
+Then-branch and else-branch do not assign the same set of variables: 
+	if 0 <= sender_index && sender_index < |s.last_checkpoi ... ... 
+
+[Action] LAcceptorProcess2a
+Harmony check failed: 
+	This output-mode variable has been assigned multiple times: 
+		s'.constants
+
+[Action] LAcceptorTruncateLog
+This expr contains an output-mode variable that is 
+	not assigned in the previous context:
+	s.(log_truncation_point := opn, votes := s'.votes)
+**********************************************************************/
+
+include ""
+
+
+module Impl_LiveRSL__Acceptor_i 
+{
+
+	datatype CAcceptor = 
+	CAcceptor(
+		constants: CReplicaConstants, 
+		max_bal: CBallot, 
+		votes: CVotes, 
+		last_checkpointed_operation: seq<COperationNumber>, 
+		log_truncation_point: COperationNumber
+	)
+
+	predicate CAcceptorIsValid(s: CAcceptor) 
+	{
+		CAcceptorIsAbstractable(s) 
+		&& 
+		CReplicaConstantsIsValid(s.constants) 
+		&& 
+		CBallotIsValid(s.max_bal) 
+		&& 
+		CVotesIsValid(s.votes) 
+		&& 
+		(forall i :: i in s.last_checkpointed_operation ==> COperationNumberIsValid(i)) 
+		&& 
+		COperationNumberIsValid(s.log_truncation_point)
+	}
+
+	predicate CAcceptorIsAbstractable(s: CAcceptor) 
+	{
+		CReplicaConstantsIsAbstractable(s.constants) 
+		&& 
+		CBallotIsAbstractable(s.max_bal) 
+		&& 
+		CVotesIsAbstractable(s.votes) 
+		&& 
+		(forall i :: i in s.last_checkpointed_operation ==> COperationNumberIsAbstractable(i)) 
+		&& 
+		COperationNumberIsAbstractable(s.log_truncation_point)
+	}
+
+	function AbstractifyCAcceptorToLAcceptor(s: CAcceptor) : LAcceptor 
+		requires CAcceptorIsAbstractable(s)
+	{
+		LAcceptor(AbstractifyCReplicaConstantsToLReplicaConstants(s.constants), AbstractifyCBallotToBallot(s.max_bal), AbstractifyCVotesToVotes(s.votes), AbstractifySeq(s.last_checkpointed_operation, AbstractifyCOperationNumberToOperationNumber), AbstractifyCOperationNumberToOperationNumber(s.log_truncation_point))
+	}
+
+	function method CAcceptorInit(c: CReplicaConstants) : CAcceptor 
+		requires CReplicaConstantsIsValid(c)
+		ensures var a := CAcceptorInit(c); CAcceptorIsValid(a) && LAcceptorInit(AbstractifyCAcceptorToLAcceptor(a), AbstractifyCReplicaConstantsToLReplicaConstants(c))
+	{
+		
+	}
+
+	function method CRemoveVotesBeforeLogTruncationPoint(votes: CVotes, log_truncation_point: COperationNumber) : CVotes 
+		requires CVotesIsValid(votes)
+		requires COperationNumberIsValid(log_truncation_point)
+		ensures var votes' := CRemoveVotesBeforeLogTruncationPoint(votes, log_truncation_point); CVotesIsValid(votes') && RemoveVotesBeforeLogTruncationPoint(AbstractifyCVotesToVotes(votes), AbstractifyCVotesToVotes(votes'), AbstractifyCOperationNumberToOperationNumber(log_truncation_point))
+	{
+		
+	}
+
+	function method CAcceptorProcessHeartbeat(s: CAcceptor, inp: CPacket) : CAcceptor 
+		requires CAcceptorIsValid(s)
+		requires CPacketIsValid(inp)
+		requires inp.msg.CMessage_Heartbeat?
+		ensures var s' := CAcceptorProcessHeartbeat(s, inp); CAcceptorIsValid(s') && LAcceptorProcessHeartbeat(AbstractifyCAcceptorToLAcceptor(s), AbstractifyCAcceptorToLAcceptor(s'), AbstractifyCPacketToRslPacket(inp))
+	{
+		
+	}
+
+	function method CAcceptorProcess2a(s: CAcceptor, inp: CPacket) : (CAcceptor, OutboundPackets) 
+		requires CAcceptorIsValid(s)
+		requires CPacketIsValid(inp)
+		requires inp.msg.CMessage_2a?
+		requires inp.src in s.constants.all.config.replica_ids
+		requires CBalLeq(s.max_bal, inp.msg.bal_2a)
+		requires CLeqUpperBound(inp.msg.opn_2a, s.constants.all.params.max_integer_val)
+		ensures var (s', broadcast_sent_packets) := CAcceptorProcess2a(s, inp); CAcceptorIsValid(s') && OutboundPacketsIsValid(broadcast_sent_packets) && LAcceptorProcess2a(AbstractifyCAcceptorToLAcceptor(s), AbstractifyCAcceptorToLAcceptor(s'), AbstractifyCPacketToRslPacket(inp), AbstractifyOutboundCPacketsToSeqOfRslPackets(broadcast_sent_packets))
+	{
+		
+	}
+
+	function method CAcceptorTruncateLog(s: CAcceptor, opn: COperationNumber) : CAcceptor 
+		requires CAcceptorIsValid(s)
+		requires COperationNumberIsValid(opn)
+		ensures var s' := CAcceptorTruncateLog(s, opn); CAcceptorIsValid(s') && LAcceptorTruncateLog(AbstractifyCAcceptorToLAcceptor(s), AbstractifyCAcceptorToLAcceptor(s'), AbstractifyCOperationNumberToOperationNumber(opn))
+	{
+		
+	}
+}
