asset/spec/BadExamples/Acceptor.i.dfy
@@ -1,0 +1,96 @@
+include "Environment.i.dfy"
+include "Configuration.i.dfy"
+include "Constants.i.dfy"
+include "Broadcast.i.dfy"
+include "../../Common/Collections/CountMatches.i.dfy"
+
+module LiveRSL__Acceptor_i {
+  import opened LiveRSL__Environment_i
+  import opened LiveRSL__Configuration_i
+  import opened LiveRSL__Constants_i
+  import opened LiveRSL__Broadcast_i
+  import opened LiveRSL__Types_i
+  import opened LiveRSL__Message_i
+  import opened Collections__CountMatches_i
+  import opened Environment_s
+  import opened Common__UpperBound_s
+
+  datatype LAcceptor = LAcceptor(
+    constants:LReplicaConstants,
+    max_bal:Ballot,
+    votes:Votes,
+    last_checkpointed_operation:seq<OperationNumber>,
+    log_truncation_point:OperationNumber
+  )
+
+  /* a.constants is not assigned */
+  predicate LAcceptorInit(a:LAcceptor, c:LReplicaConstants)
+  {
+    // && a.constants == c
+    && a.max_bal == Ballot(0,0)
+    && a.votes == map []
+    && |a.last_checkpointed_operation| == |c.all.config.replica_ids|
+    && (forall idx :: 0 <= idx < |a.last_checkpointed_operation| ==> a.last_checkpointed_operation[idx] == 0)
+    && a.log_truncation_point == 0
+  }
+
+  /* votes is not assigned as the map constructor is not complete */
+  predicate RemoveVotesBeforeLogTruncationPoint(votes:Votes, votes':Votes, log_truncation_point:OperationNumber)
+  {
+    // && (forall opn :: opn in votes' <==> opn in votes && opn >= log_truncation_point)
+    && (forall opn :: opn in votes' ==> votes'[opn] == votes[opn])
+  }
+
+  /* Then-branch and else-branch do not assign the same set of variables */ 
+  predicate LAcceptorProcessHeartbeat(s:LAcceptor, s':LAcceptor, inp:RslPacket)
+    requires inp.msg.RslMessage_Heartbeat?
+  {
+    if inp.src in s.constants.all.config.replica_ids then
+      var sender_index := GetReplicaIndex(inp.src, s.constants.all.config);
+      if 0 <= sender_index < |s.last_checkpointed_operation| && inp.msg.opn_ckpt > s.last_checkpointed_operation[sender_index] then
+        s'.last_checkpointed_operation == s.last_checkpointed_operation[sender_index := inp.msg.opn_ckpt]
+        && s'.constants == s.constants
+        && s'.max_bal == s.max_bal
+        // && s'.votes == s.votes
+        && s'.log_truncation_point == s.log_truncation_point
+      else
+        s' == s
+    else
+      s' == s
+  }
+
+  /* s'.constants assigned twice, harmony check failed */
+  predicate LAcceptorProcess2a(s:LAcceptor, s':LAcceptor, inp:RslPacket, broadcast_sent_packets:seq<RslPacket>)
+    requires inp.msg.RslMessage_2a?
+    requires inp.src in s.constants.all.config.replica_ids
+    requires BalLeq(s.max_bal, inp.msg.bal_2a)
+    requires LeqUpperBound(inp.msg.opn_2a, s.constants.all.params.max_integer_val)
+  {
+    var m := inp.msg;
+    var newLogTruncationPoint := if inp.msg.opn_2a - s.constants.all.params.max_log_length + 1 > s.log_truncation_point then
+                                   inp.msg.opn_2a - s.constants.all.params.max_log_length + 1
+                                 else
+                                   s.log_truncation_point;
+    && LBroadcastToEveryone(s.constants.all.config, s.constants.my_index, RslMessage_2b(m.bal_2a, m.opn_2a, m.val_2a), broadcast_sent_packets)
+    && s'.max_bal == m.bal_2a
+    && s'.log_truncation_point == newLogTruncationPoint
+    && (if s.log_truncation_point <= inp.msg.opn_2a then
+         LAddVoteAndRemoveOldOnes(s.votes, s'.votes, m.opn_2a, Vote(m.bal_2a, m.val_2a), newLogTruncationPoint)
+       else
+         s'.votes == s.votes
+         )
+    && s'.constants == s.constants
+    && s'.constants == 10
+    && s'.last_checkpointed_operation == s.last_checkpointed_operation
+  }
+
+  predicate LAcceptorTruncateLog(s:LAcceptor, s':LAcceptor, opn:OperationNumber)
+  {
+    if opn <= s.log_truncation_point then
+      s' == s
+    else
+      // && RemoveVotesBeforeLogTruncationPoint(s.votes, s'.votes, opn)
+      && s' == s.(log_truncation_point := opn, votes := s'.votes)
+  }
+
+}
